patch for pmac CL64

casestudy/openSSL/pmac_verify_hmac/pmac_verify_hmac_proof_BL_CL64.ec
@@ -1,72 +1,118 @@
-require import AllCore IntDiv CoreMap List.
 from Jasmin require import JModel Leakage_models.
-require Pmac_verify_hmac_ct.
+require import AllCore IntDiv CoreMap List Pmac_verify_hmac_ct.
+
 import StdOrder.IntOrder Ring.IntID.
 
-clone import Pmac_verify_hmac_ct.T with
-theory LeakageModel <-  LeakageModelCL.
+clone import Pmac_verify_hmac_ct.T with theory LeakageModel <-  LeakageModelCL.
+
+lemma invwK (c:W64.t) : invw (invw c) = c.
+proof. by apply W64.wordP => i hi; rewrite !W64.invwE hi. qed.
+
+lemma sar_and (x y:W64.t): W64.sar x 63 `&` y = if to_sint x < 0 then y else W64.zero.
+proof.
+  apply W64.wordP => i hi.
+  rewrite W64.andwE /sar W64.initiE 1:// /=.
+  have -> : min 63 (i + 63) = 63 by smt().
+  rewrite to_sintE /smod W64.get_to_uint /=.
+  have /= := W64.to_uint_cmp x; smt (W64.zerowE).
+qed.
+
+op inv (j off i:W64.t) = 
+   if to_sint j < to_sint off then to_uint i = 0
+  else if to_sint j < to_sint off + 20 then to_uint i = to_sint j - to_sint off
+  else to_uint i = 20.
+
+lemma to_sintD_small (x y : W64.t): 
+  W64.min_sint <= to_sint x + to_sint y <= W64.max_sint =>
+  to_sint (x + y) = to_sint x + to_sint y.
+proof. rewrite /W64.to_sint /smod W64.to_uintD /#. qed.
+
+lemma to_sintB_small (x y : W64.t) : 
+  W64.min_sint <= to_sint x - to_sint y <= W64.max_sint =>
+  to_sint (x - y) = to_sint x - to_sint y.
+proof. rewrite /W64.to_sint /smod W64.to_uintD to_uintNE !modzDmr /= /#. qed.
+
+lemma to_sint_small (x:int) :
+  W64.min_sint <= x <= W64.max_sint =>
+  to_sint (W64.of_int x) = x.
+proof. rewrite /to_sint /smod W64.of_uintK /= /#. qed.
+
+lemma inv_incr (len  maxpad off j i: W64.t):
+  to_uint maxpad <= 276 => 
+  to_uint len <= to_uint maxpad + 1 =>
+  off = (maxpad+ W64.one) - len => 
+  W64.to_uint j < to_uint maxpad => 
+  inv j off i =>
+  inv (j + W64.one) off
+    (i + invw (invw (j - off - W64.of_int 20 `|>>` W8.of_int 63)) `&` (off - W64.one - j `|>>` W8.of_int 63) `&` W64.one).
+proof.
+  rewrite !invwK /W64.(`|>>`) W8.to_uint_small 1:// modz_small 1://.
+  rewrite !sar_and /inv => hm hl hoff hj.
+  have sulen : to_sint len = to_uint len by rewrite /to_sint /smod /#. 
+  have suj : to_sint j = to_uint j by rewrite /to_sint /smod /#. 
+  have sumax : to_sint maxpad = to_uint maxpad by rewrite /to_sint /smod /#. 
+  have /= ?:= W64.to_uint_cmp j; have /= ?:= W64.to_uint_cmp maxpad; have /= ?:= W64.to_uint_cmp len.
+  have h1 := to_sint_small 1 _; 1 : done.
+  rewrite (to_sintD_small j W64.one) h1; 1: by rewrite /= /#.
+  have hoff' : to_sint off = (to_sint maxpad + 1) - to_sint len.
+  + by rewrite hoff to_sintB_small to_sintD_small /to_sint /smod /= // /#.
+  have -> : to_sint (j - off - W64.of_int 20) = to_sint j - to_sint off - 20.
+  + have -> : j - off - W64.of_int 20 = j - (off + W64.of_int 20) by ring.
+    have h : to_sint (off + W64.of_int 20) = to_sint off + 20.
+    + by rewrite to_sintD_small ?to_sint_small // hoff to_sintB_small to_sintD_small /= /to_sint /smod /=; smt(). 
+    rewrite to_sintB_small h hoff'; 2: by ring.
+    by rewrite /to_sint /smod /=; smt().
+  have heq : to_sint (off - W64.one - j) = to_sint off - 1 - to_sint j.
+  + have -> : off - W64.one - j = off - (W64.one + j) by ring.
+    have h : to_sint (W64.one + j) = to_sint j + 1.
+    + by rewrite to_sintD_small ?to_sint_small // /= /to_sint /smod /=; smt(). 
+    by rewrite to_sintB_small h /= /#.
+  case: (to_sint j < to_sint off) => hjoff /=.
+  + move=> hi; have -> /= : to_sint j - to_sint off - 20 < 0 by smt().
+    by rewrite sar_and heq; have -> /= /#: !(to_sint off - 1 - to_sint j < 0) by smt().
+  case: (to_sint j < to_sint off + 20) => hjoff20.
+  + have -> /= :  to_sint j - to_sint off - 20 < 0 by smt().
+    rewrite sar_and heq => hi.
+    have -> /= : !(to_sint j + 1 < to_sint off) by smt().
+    have -> /= : to_sint off - 1 - to_sint j < 0 by smt().
+    by rewrite W64.to_uintD_small /= /#. 
+  have -> /= : !(to_sint j + 1 < to_sint off) by smt().
+  have -> /= : !(to_sint j + 1 < to_sint off + 20) by smt().
+  have -> // : !(to_sint j - to_sint off - 20 < 0) by smt().
+qed.
 
 equiv l_final : M.verify_hmac_jazz ~ M.verify_hmac_jazz :
-={M.leakages, len, pmac, out, maxpad} /\
-  to_uint pmac{2} + 64 <= W64.modulus /\
-  64 %| to_uint pmac{2}
-==> ={M.leakages}.
+  ={M.leakages, pmac, maxpad} /\ (out + len){1} = (out + len){2} /\
+     to_uint pmac{2} + 64 <= W64.modulus /\ 64 %| to_uint pmac{2} /\ 
+     to_uint maxpad{1} < 256  /\
+     (to_uint len <= to_uint maxpad + 21){1} /\
+     (to_uint len <= to_uint maxpad + 21){2}
+     ==> ={M.leakages}.
 proof.
-proc; inline *; auto.
-while (={maxpad, j, p, M.leakages, len, pmac, out, maxpad} /\ to_uint pmac{2} + 64 <= W64.modulus
-        /\ 64 %| to_uint pmac{2} /\ 0 <= to_uint i{1} < 20 /\ 0 <= to_uint i{2} < 20).
-wp; skip=> />.
-+ move=> &1 &2 /= hpmac hdiv64 h0i hi20 h0i' hi20' ht.
-  rewrite /leak_mem /= /leak_mem_CL /=. split=> //=. rewrite !offset_div.
-  + by apply hpmac.
-  + by apply hdiv64.
-  + by smt().
-  + by apply hpmac.
-  + by apply hdiv64.
-  + by smt().
-  + by auto.
-  split=> //=; auto. split=> //=; auto.
-  + have hle := W64.to_uint_ule_andw ((i{1} + W64.one)%W64)
-    (zeroextu64
-    (invw (invw (truncateu32 j{2} - truncateu32 off{1} - (of_int 20)%W32 `>>`(of_int 31)%W8)))).
-    have hadd : 1 <= to_uint (i{1} + W64.one) < 21.
-    + split=> //=.
-      + rewrite to_uintD_small. + by smt().
-      rewrite /=. by smt().
-    move=> hadd'. + rewrite to_uintD_small. + by smt().
-    rewrite /=. by smt().
-    case: hadd=> hadd1 hadd2. by smt.
-  + move=> h.
-    have hle := W64.to_uint_ule_andw ((i{1} + W64.one)%W64)
-    (zeroextu64
-    (invw (invw (truncateu32 j{2} - truncateu32 off{1} - (of_int 20)%W32 `>>`(of_int 31)%W8)))).
-    have hadd : 1 <= to_uint (i{1} + W64.one) < 21.
-    + split=> //=.
-      + rewrite to_uintD_small. + by smt().
-      rewrite /=. by smt().
-    move=> hadd'. + rewrite to_uintD_small. + by smt().
-    rewrite /=. by smt().
-    admit.
-  + split=> //=; auto.
-    + have hle := W64.to_uint_ule_andw ((i{2} + W64.one)%W64)
-    (zeroextu64
-    (invw (invw (truncateu32 j{2} - truncateu32 off{2} - (of_int 20)%W32 `>>`(of_int 31)%W8)))).
-    have hadd : 1 <= to_uint (i{2} + W64.one) < 21.
-    + split=> //=.
-      + rewrite to_uintD_small. + by smt().
-      rewrite /=. by smt().
-    move=> hadd'. + rewrite to_uintD_small. + by smt().
-    rewrite /=. by smt().
-    case: hadd=> hadd1 hadd2. by smt.
-  + move=> h.
-    have hle := W64.to_uint_ule_andw ((i{2} + W64.one)%W64)
-    (zeroextu64
-    (invw (invw (truncateu32 j{2} - truncateu32 off{2} - (of_int 20)%W32 `>>`(of_int 31)%W8)))).
-    have hadd : 1 <= to_uint (i{2} + W64.one) < 21.
-    + split=> //=.
-      + rewrite to_uintD_small. + by smt().
-      rewrite /=. by smt().
-    move=> hadd'. + rewrite to_uintD_small. + by smt().
-    rewrite /=. by smt(). admit.
-wp; skip=> />.
-admitted.
+proc; wp => /=.
+while (={maxpad, j, p, M.leakages, pmac, maxpad} /\ 
+       inv j{1} off{1} i{1} /\ inv j{2} off{2} i{2} /\ 
+       to_uint j{1} <= to_uint maxpad{1} < 256 + 20 /\ 
+       to_uint pmac{2} + 64 <= W64.modulus /\ 64 %| to_uint pmac{2} /\ 
+       (off = (maxpad+ W64.one) - len){1} /\ (to_uint len <= to_uint maxpad + 1){1} /\
+       (off = (maxpad+ W64.one) - len){2} /\ (to_uint len <= to_uint maxpad + 1){2}).
++ wp; skip=> |> &1 &2 h1 h2 hjm hmax hpmac dpmac hlen1 hlen2; rewrite ultE => hj.
+  split; 1: by rewrite /leak_mem /leak_mem_CL !offset_div // 1,2:/#.
+  split; 1: by apply (inv_incr len{1} maxpad{2}) => // /#. 
+  split; 1: by apply (inv_incr len{2} maxpad{2}) => // /#. 
+  by rewrite (W64.to_uintD_small j{2} W64.one) /#.
+auto => |> &1 &2 houtlen hpmac dmac hmax hlen1 hlen2.
+rewrite {1}houtlen /= (W64.to_uintD_small maxpad{2}) /= 1:/# hlen1 hlen2 /=.
+have -> : out{1} - (out{1} + len{1} - W64.one - maxpad{2} - W64.of_int 20) = 
+          (maxpad{2} + W64.of_int 21) - len{1} by ring.
+have -> /= : out{2} - (out{2} + len{2} - W64.one - maxpad{2} - W64.of_int 20) = 
+          (maxpad{2} + W64.of_int 21) - len{2} by ring.
+have ? : to_sint (maxpad{2} + (of_int 21)%W64) = to_uint maxpad{2} + 21.
++ by rewrite to_sintD_small to_sint_small // /to_sint /smod /=; smt(W64.to_uint_cmp).
+split.
++ have ? : to_sint len{1} = to_uint len{1} by rewrite /to_sint /smod /=; smt(W64.to_uint_cmp).
+  by rewrite /inv to_sintB_small /= ?to_sint_small //; smt(W64.to_uint_cmp).
+split; last by smt(W64.to_uint_cmp).
+have ? : to_sint len{2} = to_uint len{2} by rewrite /to_sint /smod /=; smt(W64.to_uint_cmp).
+by rewrite /inv to_sintB_small /= ?to_sint_small //; smt(W64.to_uint_cmp).
+qed.
